Wrote up types and typed language

02Typed/TypedLanguage.thy
@@ -8,64 +8,94 @@ text \<open>Our typed language is almost identical to the untyped source, except
 type-annotation on every lambda-abstraction. This small change, of course, produces a great 
 difference in properties, and will take quite a lot of work to establish in the typechecking pass.\<close>
 
-inductive typecheckn :: "(var \<rightharpoonup> ty) \<Rightarrow> ty expr\<^sub>s \<Rightarrow> ty \<Rightarrow> bool" (infix "\<turnstile>\<^sub>n _ :" 50) where
-  tcn_var [simp]: "\<Gamma> x = Some t \<Longrightarrow> \<Gamma> \<turnstile>\<^sub>n Var\<^sub>s x : t"
-| tcn_const [simp]: "\<Gamma> \<turnstile>\<^sub>n Const\<^sub>s k : Num"
-| tcn_lam [simp]: "\<Gamma>(x \<mapsto> t\<^sub>1) \<turnstile>\<^sub>n e : t\<^sub>2 \<Longrightarrow> \<Gamma> \<turnstile>\<^sub>n Lam\<^sub>s x t\<^sub>1 e : Arrow t\<^sub>1 t\<^sub>2"
-| tcn_app [simp]: "\<Gamma> \<turnstile>\<^sub>n e\<^sub>1 : Arrow t\<^sub>1 t\<^sub>2 \<Longrightarrow> \<Gamma> \<turnstile>\<^sub>n e\<^sub>2 : t\<^sub>1 \<Longrightarrow> \<Gamma> \<turnstile>\<^sub>n App\<^sub>s e\<^sub>1 e\<^sub>2 : t\<^sub>2"
+text \<open>We begin with our typing relation. Thanks to the tags on binders (the only difficult part of 
+typing the lambda-calculus), we can straightforwardly check that a term has a given type. In fact, 
+we would even write it as an Isabelle function; however, since type-reconstruction is performed 
+separately and only once, and the typing judgement is only ever used to prove facts with, we go 
+with the simpler inductive relation form.\<close>
 
-inductive_cases [elim]: "\<Gamma> \<turnstile>\<^sub>n Var\<^sub>s x : t"
-inductive_cases [elim]: "\<Gamma> \<turnstile>\<^sub>n Const\<^sub>s k : t"
-inductive_cases [elim]: "\<Gamma> \<turnstile>\<^sub>n Lam\<^sub>s x t' e : t"
-inductive_cases [elim]: "\<Gamma> \<turnstile>\<^sub>n App\<^sub>s e\<^sub>1 e\<^sub>2 : t"
+inductive typing\<^sub>t :: "(var \<rightharpoonup> ty) \<Rightarrow> ty expr\<^sub>s \<Rightarrow> ty \<Rightarrow> bool" (infix "\<turnstile>\<^sub>t _ :" 50) where
+  tc\<^sub>t_var [simp]: "\<Gamma> x = Some t \<Longrightarrow> \<Gamma> \<turnstile>\<^sub>t Var\<^sub>s x : t"
+| tc\<^sub>t_const [simp]: "\<Gamma> \<turnstile>\<^sub>t Const\<^sub>s n : Num"
+| tc\<^sub>t_lam [simp]: "\<Gamma>(x \<mapsto> t\<^sub>1) \<turnstile>\<^sub>t e : t\<^sub>2 \<Longrightarrow> \<Gamma> \<turnstile>\<^sub>t Lam\<^sub>s x t\<^sub>1 e : Arrow t\<^sub>1 t\<^sub>2"
+| tc\<^sub>t_app [simp]: "\<Gamma> \<turnstile>\<^sub>t e\<^sub>1 : Arrow t\<^sub>1 t\<^sub>2 \<Longrightarrow> \<Gamma> \<turnstile>\<^sub>t e\<^sub>2 : t\<^sub>1 \<Longrightarrow> \<Gamma> \<turnstile>\<^sub>t App\<^sub>s e\<^sub>1 e\<^sub>2 : t\<^sub>2"
 
-lemma free_vars_tc [simp]: "\<Gamma> \<turnstile>\<^sub>n e : t \<Longrightarrow> free_vars\<^sub>s e \<subseteq> dom \<Gamma>" 
-  by (induction \<Gamma> e t rule: typecheckn.induct) auto
+inductive_cases [elim]: "\<Gamma> \<turnstile>\<^sub>t Var\<^sub>s x : t"
+inductive_cases [elim]: "\<Gamma> \<turnstile>\<^sub>t Const\<^sub>s n : t"
+inductive_cases [elim]: "\<Gamma> \<turnstile>\<^sub>t Lam\<^sub>s x t' e : t"
+inductive_cases [elim]: "\<Gamma> \<turnstile>\<^sub>t App\<^sub>s e\<^sub>1 e\<^sub>2 : t"
 
-lemma [simp]: "Map.empty \<turnstile>\<^sub>n e : t \<Longrightarrow> free_vars\<^sub>s e = {}"
-  using free_vars_tc by fastforce
+lemma free_vars_tc': "\<Gamma> \<turnstile>\<^sub>t e : t \<Longrightarrow> free_vars\<^sub>s e \<subseteq> dom \<Gamma>" 
+  by (induction \<Gamma> e t rule: typing\<^sub>t.induct) auto
 
-lemma canonical_base\<^sub>s [dest]: "\<Gamma> \<turnstile>\<^sub>n e : Num \<Longrightarrow> value\<^sub>s e \<Longrightarrow> \<exists>k. e = Const\<^sub>s k"
-  by (induction \<Gamma> e Num rule: typecheckn.induct) simp_all
+lemma free_vars_tc [simp]: "Map.empty \<turnstile>\<^sub>t e : t \<Longrightarrow> free_vars\<^sub>s e = {}"
+  using free_vars_tc' by fastforce
 
-lemma canonical_arrow\<^sub>s [dest]: "\<Gamma> \<turnstile>\<^sub>n e : Arrow t\<^sub>1 t\<^sub>2 \<Longrightarrow> value\<^sub>s e \<Longrightarrow> 
-    \<exists>x e'. e = Lam\<^sub>s x t\<^sub>1 e' \<and> \<Gamma>(x \<mapsto> t\<^sub>1) \<turnstile>\<^sub>n e' : t\<^sub>2"
-  by (induction \<Gamma> e "Arrow t\<^sub>1 t\<^sub>2" rule: typecheckn.induct) simp_all
+text \<open>The typing of an expression in a given context is unique:\<close>
 
-(* Progress not directly provable here, due to lack of proof of termination.
-   We prove it in 02Debruijn/NameRemoval *)
+theorem uniqueness_of_typing: "\<Gamma> \<turnstile>\<^sub>t e : t \<Longrightarrow> \<Gamma> \<turnstile>\<^sub>t e : t' \<Longrightarrow> t = t'"
+proof (induction \<Gamma> e t arbitrary: t' rule: typing\<^sub>t.induct)
+  case (tc\<^sub>t_var \<Gamma> x t)
+  from tc\<^sub>t_var(2, 1) show ?case by (induction rule: typing\<^sub>t.cases) simp_all
+next
+  case (tc\<^sub>t_const \<Gamma> n)
+  thus ?case by (induction rule: typing\<^sub>t.cases) simp_all
+next
+  case (tc\<^sub>t_lam \<Gamma> x t\<^sub>1 e t\<^sub>2)
+  from tc\<^sub>t_lam(3, 1, 2) show ?case by (induction rule: typing\<^sub>t.cases) blast+
+next
+  case (tc\<^sub>t_app \<Gamma> e\<^sub>1 t\<^sub>1 t\<^sub>2 e\<^sub>2)
+  from tc\<^sub>t_app(5, 1, 2, 3, 4) show ?case by (induction rule: typing\<^sub>t.cases) blast+
+qed
 
-lemma [simp]: "\<Gamma> \<turnstile>\<^sub>n e : t \<Longrightarrow> x \<notin> all_vars\<^sub>s e \<Longrightarrow> \<Gamma>(x \<mapsto> t') \<turnstile>\<^sub>n e : t"
-  by (induction \<Gamma> e t rule: typecheckn.induct) (simp_all add: fun_upd_twist)
+text \<open>We can also now prove the canonical-forms lemmas, telling us what shapes a well-typed value
+must have.\<close>
 
-lemma [simp]: "\<Gamma>(x \<mapsto> t') \<turnstile>\<^sub>n e : t \<Longrightarrow> x' \<notin> all_vars\<^sub>s e \<Longrightarrow> \<Gamma>(x' \<mapsto> t') \<turnstile>\<^sub>n subst_var\<^sub>s x x' e : t"
-proof (induction "\<Gamma>(x \<mapsto> t')" e t arbitrary: \<Gamma> rule: typecheckn.induct)
-  case (tcn_lam y t\<^sub>1 e t\<^sub>2)
+lemma canonical_num [dest]: "\<Gamma> \<turnstile>\<^sub>t e : Num \<Longrightarrow> value\<^sub>s e \<Longrightarrow> \<exists>n. e = Const\<^sub>s n"
+  by (induction \<Gamma> e Num rule: typing\<^sub>t.induct) simp_all
+
+lemma canonical_arrow\<^sub>t [dest]: "\<Gamma> \<turnstile>\<^sub>t e : Arrow t\<^sub>1 t\<^sub>2 \<Longrightarrow> value\<^sub>s e \<Longrightarrow> 
+    \<exists>x e'. e = Lam\<^sub>s x t\<^sub>1 e' \<and> \<Gamma>(x \<mapsto> t\<^sub>1) \<turnstile>\<^sub>t e' : t\<^sub>2"
+  by (induction \<Gamma> e "Arrow t\<^sub>1 t\<^sub>2" rule: typing\<^sub>t.induct) simp_all
+
+text \<open>Finally, we can prove the preservation theorem, one half of the traditional formulation of
+language safety. The other half, progress, is true of our language at this point, now that we have 
+restricted our sights to the typed subset; but our complex capture-avoiding substitution operation 
+would make proving it more painful than necessary. We will return to it once we have moved to a 
+Debruijn variable representation.\<close>
+
+lemma tc\<^sub>t_widen_context [simp]: "\<Gamma> \<turnstile>\<^sub>t e : t \<Longrightarrow> x \<notin> all_vars\<^sub>s e \<Longrightarrow> \<Gamma>(x \<mapsto> t') \<turnstile>\<^sub>t e : t"
+  by (induction \<Gamma> e t rule: typing\<^sub>t.induct) (simp_all add: fun_upd_twist)
+
+lemma tc\<^sub>t_subst_var [simp]: "\<Gamma>(x \<mapsto> t') \<turnstile>\<^sub>t e : t \<Longrightarrow> x' \<notin> all_vars\<^sub>s e \<Longrightarrow> 
+  \<Gamma>(x' \<mapsto> t') \<turnstile>\<^sub>t subst_var\<^sub>s x x' e : t"
+proof (induction "\<Gamma>(x \<mapsto> t')" e t arbitrary: \<Gamma> rule: typing\<^sub>t.induct)
+  case (tc\<^sub>t_lam y t\<^sub>1 e t\<^sub>2)
   thus ?case
   proof (cases "x = y")
     case False
-    moreover with tcn_lam have "\<Gamma>(y \<mapsto> t\<^sub>1, x' \<mapsto> t') \<turnstile>\<^sub>n subst_var\<^sub>s x x' e : t\<^sub>2" 
+    moreover with tc\<^sub>t_lam have "\<Gamma>(y \<mapsto> t\<^sub>1, x' \<mapsto> t') \<turnstile>\<^sub>t subst_var\<^sub>s x x' e : t\<^sub>2" 
       by (simp add: fun_upd_twist)
-    moreover from tcn_lam have "x' \<noteq> y" by simp
+    moreover from tc\<^sub>t_lam have "x' \<noteq> y" by simp
     ultimately show ?thesis by (simp add: fun_upd_twist)
   qed (simp_all add: fun_upd_twist)
 qed fastforce+
 
-lemma [simp]: "\<Gamma>(x \<mapsto> t') \<turnstile>\<^sub>n e : t \<Longrightarrow> \<Gamma> \<turnstile>\<^sub>n e' : t' \<Longrightarrow> \<Gamma> \<turnstile>\<^sub>n subst\<^sub>s x e' e : t"
+lemma tc\<^sub>t_subst [simp]: "\<Gamma>(x \<mapsto> t') \<turnstile>\<^sub>t e : t \<Longrightarrow> \<Gamma> \<turnstile>\<^sub>t e' : t' \<Longrightarrow> \<Gamma> \<turnstile>\<^sub>t subst\<^sub>s x e' e : t"
 proof (induction x e' e arbitrary: \<Gamma> t rule: subst\<^sub>s.induct)
   case (3 x e' y t\<^sub>1 e)
-  then obtain t\<^sub>2 where T: "t = Arrow t\<^sub>1 t\<^sub>2 \<and> \<Gamma>(x \<mapsto> t', y \<mapsto> t\<^sub>1) \<turnstile>\<^sub>n e : t\<^sub>2" by blast
+  then obtain t\<^sub>2 where T: "t = Arrow t\<^sub>1 t\<^sub>2 \<and> \<Gamma>(x \<mapsto> t', y \<mapsto> t\<^sub>1) \<turnstile>\<^sub>t e : t\<^sub>2" by blast
   let ?z = "fresh (all_vars\<^sub>s e' \<union> all_vars\<^sub>s e \<union> {x, y})"
   have "finite (all_vars\<^sub>s e' \<union> all_vars\<^sub>s e \<union> {x, y})" by simp
   hence Z: "?z \<notin> all_vars\<^sub>s e' \<union> all_vars\<^sub>s e \<union> {x, y}" by (metis fresh_is_fresh)
-  with T have "\<Gamma>(x \<mapsto> t', ?z \<mapsto> t\<^sub>1) \<turnstile>\<^sub>n subst_var\<^sub>s y ?z e : t\<^sub>2" by simp
-  with Z have X: "\<Gamma>(?z \<mapsto> t\<^sub>1, x \<mapsto> t') \<turnstile>\<^sub>n subst_var\<^sub>s y ?z e : t\<^sub>2" by (simp add: fun_upd_twist)
-  from 3 Z have "\<Gamma>(?z \<mapsto> t\<^sub>1) \<turnstile>\<^sub>n e' : t'" by simp
-  with 3 X have "\<Gamma>(?z \<mapsto> t\<^sub>1) \<turnstile>\<^sub>n subst\<^sub>s x e' (subst_var\<^sub>s y ?z e) : t\<^sub>2" by fastforce
+  with T have "\<Gamma>(x \<mapsto> t', ?z \<mapsto> t\<^sub>1) \<turnstile>\<^sub>t subst_var\<^sub>s y ?z e : t\<^sub>2" by simp
+  with Z have X: "\<Gamma>(?z \<mapsto> t\<^sub>1, x \<mapsto> t') \<turnstile>\<^sub>t subst_var\<^sub>s y ?z e : t\<^sub>2" by (simp add: fun_upd_twist)
+  from 3 Z have "\<Gamma>(?z \<mapsto> t\<^sub>1) \<turnstile>\<^sub>t e' : t'" by simp
+  with 3 X have "\<Gamma>(?z \<mapsto> t\<^sub>1) \<turnstile>\<^sub>t subst\<^sub>s x e' (subst_var\<^sub>s y ?z e) : t\<^sub>2" by fastforce
   with T show ?case by (simp add: Let_def)
 qed fastforce+
 
-theorem preservationn: "e \<Down> v \<Longrightarrow> \<Gamma> \<turnstile>\<^sub>n e : t \<Longrightarrow> \<Gamma> \<turnstile>\<^sub>n v : t"
+theorem preservation\<^sub>t: "e \<Down> v \<Longrightarrow> \<Gamma> \<turnstile>\<^sub>t e : t \<Longrightarrow> \<Gamma> \<turnstile>\<^sub>t v : t"
   by (induction e v arbitrary: t rule: eval\<^sub>s.induct) fastforce+
 
 end
