02Typed/Type.thy
@@ -2,6 +2,11 @@ theory Type
   imports "../00Utils/Variable"
 begin
 
+section \<open>Typed language\<close>
+
+text \<open>Now we are ready to begin typechecking our source language. Since we use only simple types, 
+with no free or even bound type variables, this is quite quick.\<close>
+
 datatype ty = 
   Num 
   | Arrow ty ty
